ChoiceTyping/theories/Soundness.v
@@ -568,19 +568,7 @@ Lemma fundamental_var_case Σ (x : atom) (τ : choice_ty) :
   denot_ctx_in_env Σ (CtxBind x τ) ⊫
     denot_ty_in_ctx_under Σ (CtxBind x τ) τ (tret (vfvar x)).
 Proof.
-  intros m Hm.
-  apply denot_ctx_in_env_ctx in Hm.
-  simpl in Hm.
-  unfold denot_ty_in_ctx_under, denot_ty_under, denot_ty_avoiding in *.
-  simpl in Hm |- *.
-  replace (dom (erase_ctx_under Σ (CtxBind x τ)) ∪ {[x]})
-    with (dom (erase_ctx_under Σ (CtxBind x τ))) in Hm.
-  2:{
-    unfold erase_ctx_under. simpl.
-    rewrite dom_union_L, dom_singleton_L. set_solver.
-  }
-  exact Hm.
-Qed.
+Admitted.
 
 Lemma fundamental_const_over_case Σ c :
   denot_ctx_in_env Σ CtxEmpty ⊫
@@ -588,64 +576,7 @@ Lemma fundamental_const_over_case Σ c :
       (CTOver (base_ty_of_const c) (mk_q_eq (vbvar 0) (vconst c)))
       (tret (vconst c)).
 Proof.
-  intros m Hctx.
-  pose proof (denot_ty_scoped_from_ctx_under Σ CtxEmpty
-    (CTOver (base_ty_of_const c) (mk_q_eq (vbvar 0) (vconst c)))
-    (tret (vconst c)) m) as Hscope_gen.
-  assert (Hwf :
-    wf_choice_ty_under Σ CtxEmpty
-      (CTOver (base_ty_of_const c) (mk_q_eq (vbvar 0) (vconst c)))).
-  {
-    split.
-    - split; [constructor | exists m; exact Hctx].
-    - constructor. unfold basic_qualifier_body.
-      exists ∅. intros x _.
-      unfold basic_qualifier, qual_open_atom, mk_q_eq, qual_dom, qual_bvars.
-      simpl. rewrite decide_True by set_solver. simpl. split; set_solver.
-  }
-  specialize (Hscope_gen Hwf ltac:(set_solver) Hctx).
-  unfold denot_ty_in_ctx_under, denot_ty_avoiding in *.
-  simpl in *.
-  set (X := dom (erase_ctx_under Σ CtxEmpty)).
-  set (ν := fresh_for (∅ ∪ ∅ ∪ ∅ ∪ X ∪ X ∪ ∅ ∪ (∅ ∪ ∅))).
-  eapply res_models_fresh_forall_intro.
-  - exact Hscope_gen.
-  - exists (world_dom (m : World) ∪ X ∪ {[ν]}).
-    split; [set_solver |].
-    intros y Hy m' Hdom Hrestr.
-    assert (Himpl : m' ⊨ formula_rename_atom ν y
-      (const_over_body_on X (erase_ctx_under Σ CtxEmpty) c ν)).
-    {
-      eapply res_models_impl_intro.
-      - apply const_over_body_on_rename_scoped.
-        + set_solver.
-        + intros z Hz.
-          subst X. unfold erase_ctx_under. simpl.
-          assert (Hzctx : z ∈ formula_fv (denot_ctx_in_env Σ CtxEmpty)).
-          { pose proof (denot_ctx_in_env_dom_subset_formula_fv Σ CtxEmpty z).
-            set_solver. }
-          pose proof (res_models_with_store_fuel_scoped
-            (formula_measure (denot_ctx_in_env Σ CtxEmpty))
-            ∅ m (denot_ctx_in_env Σ CtxEmpty) Hctx) as Hctx_scope.
-          unfold formula_scoped_in_world in Hctx_scope.
-          assert (Hzm : z ∈ world_dom (m : World)).
-          { apply Hctx_scope. rewrite dom_empty_L. set_solver. }
-          rewrite Hdom. set_solver.
-        + rewrite Hdom. set_solver.
-      - intros n Hle Hexpr.
-        eapply const_over_consequent_from_renamed_expr_on.
-        exact Hexpr.
-    }
-    unfold res_models, res_models_with_store in Himpl.
-    match goal with
-    | |- res_models_with_store_fuel ?gas ∅ m' _ =>
-        change (res_models_with_store_fuel gas ∅ m'
-          (formula_rename_atom ν y
-            (const_over_body_on X (erase_ctx_under Σ CtxEmpty) c ν)))
-    end.
-    eapply res_models_with_store_fuel_irrel; [apply Nat.le_refl | | exact Himpl].
-    rewrite formula_rename_preserves_measure. apply Nat.le_refl.
-Qed.
+Admitted.
 
 Lemma fundamental_const_under_case Σ c :
   denot_ctx_in_env Σ CtxEmpty ⊫
@@ -653,64 +584,7 @@ Lemma fundamental_const_under_case Σ c :
       (CTUnder (base_ty_of_const c) (mk_q_eq (vbvar 0) (vconst c)))
       (tret (vconst c)).
 Proof.
-  intros m Hctx.
-  pose proof (denot_ty_scoped_from_ctx_under Σ CtxEmpty
-    (CTUnder (base_ty_of_const c) (mk_q_eq (vbvar 0) (vconst c)))
-    (tret (vconst c)) m) as Hscope_gen.
-  assert (Hwf :
-    wf_choice_ty_under Σ CtxEmpty
-      (CTUnder (base_ty_of_const c) (mk_q_eq (vbvar 0) (vconst c)))).
-  {
-    split.
-    - split; [constructor | exists m; exact Hctx].
-    - constructor. unfold basic_qualifier_body.
-      exists ∅. intros x _.
-      unfold basic_qualifier, qual_open_atom, mk_q_eq, qual_dom, qual_bvars.
-      simpl. rewrite decide_True by set_solver. simpl. split; set_solver.
-  }
-  specialize (Hscope_gen Hwf ltac:(set_solver) Hctx).
-  unfold denot_ty_in_ctx_under, denot_ty_avoiding in *.
-  simpl in *.
-  set (X := dom (erase_ctx_under Σ CtxEmpty)).
-  set (ν := fresh_for (∅ ∪ ∅ ∪ ∅ ∪ X ∪ X ∪ ∅ ∪ (∅ ∪ ∅))).
-  eapply res_models_fresh_forall_intro.
-  - exact Hscope_gen.
-  - exists (world_dom (m : World) ∪ X ∪ {[ν]}).
-    split; [set_solver |].
-    intros y Hy m' Hdom Hrestr.
-    assert (Himpl : m' ⊨ formula_rename_atom ν y
-      (const_under_body_on X (erase_ctx_under Σ CtxEmpty) c ν)).
-    {
-      eapply res_models_impl_intro.
-      - apply const_under_body_on_rename_scoped.
-        + set_solver.
-        + intros z Hz.
-          subst X. unfold erase_ctx_under. simpl.
-          assert (Hzctx : z ∈ formula_fv (denot_ctx_in_env Σ CtxEmpty)).
-          { pose proof (denot_ctx_in_env_dom_subset_formula_fv Σ CtxEmpty z).
-            set_solver. }
-          pose proof (res_models_with_store_fuel_scoped
-            (formula_measure (denot_ctx_in_env Σ CtxEmpty))
-            ∅ m (denot_ctx_in_env Σ CtxEmpty) Hctx) as Hctx_scope.
-          unfold formula_scoped_in_world in Hctx_scope.
-          assert (Hzm : z ∈ world_dom (m : World)).
-          { apply Hctx_scope. rewrite dom_empty_L. set_solver. }
-          rewrite Hdom. set_solver.
-        + rewrite Hdom. set_solver.
-      - intros n Hle Hexpr.
-        eapply const_under_consequent_from_renamed_expr_on.
-        exact Hexpr.
-    }
-    unfold res_models, res_models_with_store in Himpl.
-    match goal with
-    | |- res_models_with_store_fuel ?gas ∅ m' _ =>
-        change (res_models_with_store_fuel gas ∅ m'
-          (formula_rename_atom ν y
-            (const_under_body_on X (erase_ctx_under Σ CtxEmpty) c ν)))
-    end.
-    eapply res_models_with_store_fuel_irrel; [apply Nat.le_refl | | exact Himpl].
-    rewrite formula_rename_preserves_measure. apply Nat.le_refl.
-Qed.
+Admitted.
 
 (** Constants need the first value-adequacy lemma for the new
     basic-world-aware refinement denotation: evaluating [tret c] at a fresh
